3.1={n-}3.1{-n}
3.2(b)={n-}3.2(b){-n}
3.2(c)={n-}3.2(c){-n}
3.10={n-}3.10{-n}
3.11(a)={n-}3.11(a){-n}
3.11(b)={n-}3.11(b){-n}
3.11(e)={n-}3.11(e){-n}
3.13(a)={n-}3.13(a){-n}
3.13(c)={n-}3.13(c){-n}
3.14(a)={n-}3.14(a){-n}
3.14(b)={n-}3.14(b){-n}
3.15(a)={n-}3.15(a){-n}
3.15(b)={n-}3.15(b){-n}
3.15(c)={n-}3.15(c){-n}
3.16={n-}3.16{-n}
3.17(a)(v)={n-}3.17(a)(v){-n}
3.17(a)={n-}3.17(a){-n}
3.17(b)={n-}3.17(b){-n}
3.17(c)={n-}3.17(c){-n}
3.18(a)={n-}3.18(a){-n}
3.18(c)={n-}3.18(c){-n}
3.18(d)={n-}3.18(d){-n}
3.18(f)={n-}3.18(f){-n}
3.19={n-}3.19{-n}
3.20(a)={n-}3.20(a){-n}
3.20(b)={n-}3.20(b){-n}
3.20(c)={n-}3.20(c){-n}
3.20(d)={n-}3.20(d){-n}
3.20(e)={n-}3.20(e){-n}
3.22(c)={n-}3.22(c){-n}
3.22(d)={n-}3.22(d){-n}
3.22(e)={n-}3.22(e){-n}
3.22(h)={n-}3.22(h){-n}
3.24={n-}3.24{-n}
3.26={n-}3.26{-n}
3.27(b)={n-}3.27(b){-n}
3.3(a)={n-}3.3(a){-n}
3.3(b)={n-}3.3(b){-n}
3.6(a)={n-}3.6(a){-n}
3.6(b)={n-}3.6(b){-n}
3.6(c)={n-}3.6(c){-n}
3.6(d)={n-}3.6(d){-n}
3.8={n-}3.8{-n}
3.9={n-}3.9{-n}

n-=<a><font color="blue">

-n=</font><a>

